Pass through Coinductive up to PL example

src/Coinductive.v
@@ -1,4 +1,4 @@
-(* Copyright (c) 2008-2010, Adam Chlipala
+(* Copyright (c) 2008-2011, Adam Chlipala
  * 
  * This work is licensed under a
  * Creative Commons Attribution-Noncommercial-No Derivative Works 3.0
@@ -18,15 +18,13 @@ Set Implicit Arguments.
 
 (** %\chapter{Infinite Data and Proofs}% *)
 
-(** In lazy functional programming languages like Haskell, infinite data structures are everywhere.  Infinite lists and more exotic datatypes provide convenient abstractions for communication between parts of a program.  Achieving similar convenience without infinite lazy structures would, in many cases, require acrobatic inversions of control flow.
+(** In lazy functional programming languages like %\index{Haskell}%Haskell, infinite data structures are everywhere.  Infinite lists and more exotic datatypes provide convenient abstractions for communication between parts of a program.  Achieving similar convenience without infinite lazy structures would, in many cases, require acrobatic inversions of control flow.
 
-Laziness is easy to implement in Haskell, where all the definitions in a program may be thought of as mutually recursive.  In such an unconstrained setting, it is easy to implement an infinite loop when you really meant to build an infinite list, where any finite prefix of the list should be forceable in finite time.  Haskell programmers learn how to avoid such slip-ups.  In Coq, such a laissez-faire policy is not good enough.
+%\index{laziness}%Laziness is easy to implement in Haskell, where all the definitions in a program may be thought of as mutually recursive.  In such an unconstrained setting, it is easy to implement an infinite loop when you really meant to build an infinite list, where any finite prefix of the list should be forceable in finite time.  Haskell programmers learn how to avoid such slip-ups.  In Coq, such a laissez-faire policy is not good enough.
 
-We spent some time in the last chapter discussing the Curry-Howard isomorphism, where proofs are identified with functional programs.  In such a setting, infinite loops, intended or otherwise, are disastrous.  If Coq allowed the full breadth of definitions that Haskell did, we could code up an infinite loop and use it to prove any proposition vacuously.  That is, the addition of general recursion would make CIC %\textit{%#<i>#inconsistent#</i>#%}%.  For an arbitrary proposition [P], we could write:
-
+We spent some time in the last chapter discussing the %\index{Curry-Howard correspondence}%Curry-Howard isomorphism, where proofs are identified with functional programs.  In such a setting, infinite loops, intended or otherwise, are disastrous.  If Coq allowed the full breadth of definitions that Haskell did, we could code up an infinite loop and use it to prove any proposition vacuously.  That is, the addition of general recursion would make CIC %\textit{%#<i>#inconsistent#</i>#%}%.  For an arbitrary proposition [P], we could write:
 [[
 Fixpoint bad (u : unit) : P := bad u.
- 
 ]]
 
 This would leave us with [bad tt] as a proof of [P].
@@ -35,12 +33,12 @@ There are also algorithmic considerations that make universal termination very d
 
 One solution is to use types to contain the possibility of non-termination.  For instance, we can create a %``%#"#non-termination monad,#"#%''% inside which we must write all of our general-recursive programs.  This is a heavyweight solution, and so we would like to avoid it whenever possible.
 
-Luckily, Coq has special support for a class of lazy data structures that happens to contain most examples found in Haskell.  That mechanism, %\textit{%#<i>#co-inductive types#</i>#%}%, is the subject of this chapter. *)
+Luckily, Coq has special support for a class of lazy data structures that happens to contain most examples found in Haskell.  That mechanism, %\index{co-inductive types}\textit{%#<i>#co-inductive types#</i>#%}%, is the subject of this chapter. *)
 
 
 (** * Computing with Infinite Data *)
 
-(** Let us begin with the most basic type of infinite data, %\textit{%#<i>#streams#</i>#%}%, or lazy lists. *)
+(** Let us begin with the most basic type of infinite data, %\textit{%#<i>#streams#</i>#%}%, or lazy lists.%\index{Vernacular commands!CoInductive}% *)
 
 Section stream.
   Variable A : Set.
@@ -51,18 +49,25 @@ End stream.
 
 (** The definition is surprisingly simple.  Starting from the definition of [list], we just need to change the keyword [Inductive] to [CoInductive].  We could have left a [Nil] constructor in our definition, but we will leave it out to force all of our streams to be infinite.
 
-   How do we write down a stream constant?  Obviously simple application of constructors is not good enough, since we could only denote finite objects that way.  Rather, whereas recursive definitions were necessary to %\textit{%#<i>#use#</i>#%}% values of recursive inductive types effectively, here we find that we need %\textit{%#<i>#co-recursive definitions#</i>#%}% to %\textit{%#<i>#build#</i>#%}% values of co-inductive types effectively.
+   How do we write down a stream constant?  Obviously simple application of constructors is not good enough, since we could only denote finite objects that way.  Rather, whereas recursive definitions were necessary to %\textit{%#<i>#use#</i>#%}% values of recursive inductive types effectively, here we find that we need %\index{co-recursive definitions}\textit{%#<i>#co-recursive definitions#</i>#%}% to %\textit{%#<i>#build#</i>#%}% values of co-inductive types effectively.
 
-   We can define a stream consisting only of zeroes. *)
+   We can define a stream consisting only of zeroes.%\index{Vernacular commands!CoFixpoint}% *)
 
 CoFixpoint zeroes : stream nat := Cons 0 zeroes.
 
+(* EX: Define a stream that alternates between [true] and [false]. *)
+(* begin thide *)
+
 (** We can also define a stream that alternates between [true] and [false]. *)
 
-CoFixpoint trues : stream bool := Cons true falses
-with falses : stream bool := Cons false trues.
+CoFixpoint trues_falses : stream bool := Cons true falses_trues
+with falses_trues : stream bool := Cons false trues_falses.
+(* end thide *)
 
 (** Co-inductive values are fair game as arguments to recursive functions, and we can use that fact to write a function to take a finite approximation of a stream. *)
+
+(* EX: Defint a function to calculate a finite approximation of a stream, to a particular length. *)
+(* begin thide *)
 
 Fixpoint approx A (s : stream A) (n : nat) : list A :=
   match n with
@@ -80,7 +85,7 @@ Eval simpl in approx zeroes 10.
      ]]
      *)
 
-Eval simpl in approx trues 10.
+Eval simpl in approx trues_falses 10.
 (** %\vspace{-.15in}% [[
      = true
        :: false
@@ -88,28 +93,30 @@ Eval simpl in approx trues 10.
              :: false
                 :: true :: false :: true :: false :: true :: false :: nil
      : list bool
- 
-     ]]
+      ]]
+*)
 
-     So far, it looks like co-inductive types might be a magic bullet, allowing us to import all of the Haskeller's usual tricks.  However, there are important restrictions that are dual to the restrictions on the use of inductive types.  Fixpoints %\textit{%#<i>#consume#</i>#%}% values of inductive types, with restrictions on which %\textit{%#<i>#arguments#</i>#%}% may be passed in recursive calls.  Dually, co-fixpoints %\textit{%#<i>#produce#</i>#%}% values of co-inductive types, with restrictions on what may be done with the %\textit{%#<i>#results#</i>#%}% of co-recursive calls.
+(* end thide *) 
 
-The restriction for co-inductive types shows up as the %\textit{%#<i>#guardedness condition#</i>#%}%, and it can be broken into two parts.  First, consider this stream definition, which would be legal in Haskell.
+(** So far, it looks like co-inductive types might be a magic bullet, allowing us to import all of the Haskeller's usual tricks.  However, there are important restrictions that are dual to the restrictions on the use of inductive types.  Fixpoints %\textit{%#<i>#consume#</i>#%}% values of inductive types, with restrictions on which %\textit{%#<i>#arguments#</i>#%}% may be passed in recursive calls.  Dually, co-fixpoints %\textit{%#<i>#produce#</i>#%}% values of co-inductive types, with restrictions on what may be done with the %\textit{%#<i>#results#</i>#%}% of co-recursive calls.
 
+The restriction for co-inductive types shows up as the %\index{guardedness condition}\textit{%#<i>#guardedness condition#</i>#%}%, and it can be broken into two parts.  First, consider this stream definition, which would be legal in Haskell.
 [[
 CoFixpoint looper : stream nat := looper.
+]]
 
+<<
 Error:
 Recursive definition of looper is ill-formed.
 In environment
 looper : stream nat
 
 unguarded recursive call in "looper"
- 
-]]
+>>
 
 The rule we have run afoul of here is that %\textit{%#<i>#every co-recursive call must be guarded by a constructor#</i>#%}%; that is, every co-recursive call must be a direct argument to a constructor of the co-inductive type we are generating.  It is a good thing that this rule is enforced.  If the definition of [looper] were accepted, our [approx] function would run forever when passed [looper], and we would have fallen into inconsistency.
 
-The second rule of guardedness is easiest to see by first introducing a more complicated, but legal, co-fixpoint. *)
+Some familiar functions are easy to write in co-recursive fashion. *)
 
 Section map.
   Variables A B : Set.
@@ -121,9 +128,9 @@ Section map.
     end.
 End map.
 
-(** This code is a literal copy of that for the list [map] function, with the [Nil] case removed and [Fixpoint] changed to [CoFixpoint].  Many other standard functions on lazy data structures can be implemented just as easily.  Some, like [filter], cannot be implemented.  Since the predicate passed to [filter] may reject every element of the stream, we cannot satisfy even the first guardedness condition.
+(** This code is a literal copy of that for the list [map] function, with the [Nil] case removed and [Fixpoint] changed to [CoFixpoint].  Many other standard functions on lazy data structures can be implemented just as easily.  Some, like [filter], cannot be implemented.  Since the predicate passed to [filter] may reject every element of the stream, we cannot satisfy the guardedness condition.
 
-   The second condition is subtler.  To illustrate it, we start off with another co-recursive function definition that %\textit{%#<i>#is#</i>#%}% legal.  The function [interleave] takes two streams and produces a new stream that alternates between their elements. *)
+   The implications of the condition can be subtle.  To illustrate how, we start off with another co-recursive function definition that %\textit{%#<i>#is#</i>#%}% legal.  The function [interleave] takes two streams and produces a new stream that alternates between their elements. *)
 
 Section interleave.
   Variable A : Set.
@@ -143,17 +150,43 @@ Section map'.
   (** [[
   CoFixpoint map' (s : stream A) : stream B :=
     match s with
-      | Cons h t => interleave (Cons (f h) (map' t) (Cons (f h) (map' t))
+      | Cons h t => interleave (Cons (f h) (map' t)) (Cons (f h) (map' t))
     end.
- 
     ]]
     
-    We get another error message about an unguarded recursive call.  This is because we are violating the second guardedness condition, which says that, not only must co-recursive calls be arguments to constructors, there must also %\textit{%#<i>#not be anything but [match]es and calls to constructors of the same co-inductive type#</i>#%}% wrapped around these immediate uses of co-recursive calls.  The actual implemented rule for guardedness is a little more lenient than what we have just stated, but you can count on the illegality of any exception that would enhance the expressive power of co-recursion.
-
-     Why enforce a rule like this?  Imagine that, instead of [interleave], we had called some other, less well-behaved function on streams.  Perhaps this other function might be defined mutually with [map'].  It might deconstruct its first argument, retrieving [map' t] from within [Cons (f h) (map' t)].  Next it might try a [match] on this retrieved value, which amounts to deconstructing [map' t].  To figure out how this [match] turns out, we need to know the top-level structure of [map' t], but this is exactly what we started out trying to determine!  We run into a loop in the evaluation process, and we have reached a witness of inconsistency if we are evaluating [approx (map' s) 1] for any [s]. *)
-(* end thide *)
+    We get another error message about an unguarded recursive call. *)
 
 End map'.
+
+(** What is going wrong here?  Imagine that, instead of [interleave], we had called some other, less well-behaved function on streams.  Here is one simpler example demonstrating the essential pitfall.  We start defining a standard function for taking the tail of a stream.  Since streams are infinite, this operation is total. *)
+
+Definition tl A (s : stream A) : stream A :=
+  match s with
+    | Cons _ s' => s'
+  end.
+
+(** Coq rejects the following definition that uses [tl].
+[[
+CoFixpoint bad : stream nat := tl (Cons 0 bad).
+]]
+
+Imagine that Coq had accepted our definition, and consider how we might evaluate [approx bad 1].  We would be trying to calculate the first element in the stream [bad].  However, it is not hard to see that the definition of [bad] %``%#"#begs the question#"#%''%: unfolding the definition of [tl], we see that we essentially say %``%#"#define [bad] to equal itself#"#%''%!  Of course such an equation admits no single well-defined solution, which does not fit well with the determinism of Gallina reduction.
+
+Since Coq can be considered to check definitions after inlining and simplification of previously defined identifiers, the basic guardedness condition rules out our definition of [bad].  Such an inlining reduces [bad] to:
+[[
+CoFixpoint bad : stream nat := bad.
+]]
+This is the same looping definition we rejected earlier.  A similar inlining process reveals the way that Coq saw our failed definition of [map']:
+[[
+CoFixpoint map' (s : stream A) : stream B :=
+  match s with
+    | Cons h t => Cons (f h) (Cons (f h) (interleave (map' t) (map' t)))
+  end.
+]]
+Clearly in this case the [map'] calls are not immediate arguments to constructors, so we violate the guardedness condition. *)
+(* end thide *)
+
+(** A more interesting question is why that condition is the right one.  We can make an intuitive argument that the original [map'] definition is perfectly reasonable and denotes a well-understood transformation on streams, such that every output would behave properly with [approx].  The guardedness condition is an example of a syntactic check for %\index{productivity}\emph{%#<i>#productivity#</i>#%}% of co-recursive definitions.  A productive definition can be thought of as one whose outputs can be forced in finite time to any finite approximation level, as with [approx].  If we replaced the guardedness condition with more involved checks, we might be able to detect and allow a broader range of productive definitions.  However, mistakes in these checks could cause inconsistency, and programmers would need to understand the new, more complex checks.  Coq's design strikes a balance between consistency and simplicity with its choice of guard condition, though we can imagine other worthwhile balances being struck, too. *)
 
 
 (** * Infinite Proofs *)
@@ -174,7 +207,7 @@ Abort.
 
 (** Co-inductive datatypes make sense by analogy from Haskell.  What we need now is a %\textit{%#<i>#co-inductive proposition#</i>#%}%.  That is, we want to define a proposition whose proofs may be infinite, subject to the guardedness condition.  The idea of infinite proofs does not show up in usual mathematics, but it can be very useful (unsurprisingly) for reasoning about infinite data structures.  Besides examples from Haskell, infinite data and proofs will also turn out to be useful for modelling inherently infinite mathematical objects, like program executions.
 
-We are ready for our first co-inductive predicate. *)
+We are ready for our first %\index{co-inductive predicates}%co-inductive predicate. *)
 
 Section stream_eq.
   Variable A : Set.
@@ -205,14 +238,14 @@ Theorem ones_eq : stream_eq ones ones'.
   assumption.
   (** [[
 Proof completed.
- 
 ]]
 
   Unfortunately, we are due for some disappointment in our victory lap.
-
   [[
 Qed.
+]]
 
+<<
 Error:
 Recursive definition of ones_eq is ill-formed.
 
@@ -220,16 +253,13 @@ In environment
 ones_eq : stream_eq ones ones'
 
 unguarded recursive call in "ones_eq"
- 
-]]
+>>
 
 Via the Curry-Howard correspondence, the same guardedness condition applies to our co-inductive proofs as to our co-inductive data structures.  We should be grateful that this proof is rejected, because, if it were not, the same proof structure could be used to prove any co-inductive theorem vacuously, by direct appeal to itself!
 
-Thinking about how Coq would generate a proof term from the proof script above, we see that the problem is that we are violating the first part of the guardedness condition.  During our proofs, Coq can help us check whether we have yet gone wrong in this way.  We can run the command [Guarded] in any context to see if it is possible to finish the proof in a way that will yield a properly guarded proof term.
-
+Thinking about how Coq would generate a proof term from the proof script above, we see that the problem is that we are violating the guardedness condition.  During our proofs, Coq can help us check whether we have yet gone wrong in this way.  We can run the command [Guarded] in any context to see if it is possible to finish the proof in a way that will yield a properly guarded proof term.%\index{Vernacular command!Guarded}%
      [[
 Guarded.
-
 ]]
 
      Running [Guarded] here gives us the same error message that we got when we tried to run [Qed].  In larger proofs, [Guarded] can be helpful in detecting problems %\textit{%#<i>#before#</i>#%}% we think we are ready to run [Qed].
@@ -293,7 +323,7 @@ Theorem ones_eq : stream_eq ones ones'.
  
             ]]
 
-  Since we have exposed the [Cons] structure of each stream, we can apply the constructor of [stream_eq]. *)
+  Note that [cofix] notation for anonymous co-recursion, which is analogous to the [fix] notation we have already seen for recursion.  Since we have exposed the [Cons] structure of each stream, we can apply the constructor of [stream_eq]. *)
 
   constructor.
   (** [[
@@ -324,13 +354,165 @@ Theorem ones_eq' : stream_eq ones ones'.
   cofix; crush.
   (** [[
   Guarded.
-
   ]]
   *)
 Abort.
+
+(** The standard [auto] machinery sees that our goal matches an assumption and so applies that assumption, even though this violates guardedness.  One usually starts a proof like this by [destruct]ing some parameter and running a custom tactic to figure out the first proof rule to apply for each case.  Alternatively, there are tricks that can be played with %``%#"#hiding#"#%''% the co-inductive hypothesis.
+
+   %\medskip%
+
+   Must we always be cautious with automation in proofs by co-induction?  Induction seems to have dual versions the same pitfalls inherent in it, and yet we avoid those pitfalls by encapsulating safe Curry-Howard recursion schemes inside named induction principles.  It turns out that we can usually do the same with %\index{co-induction principles}\emph{%#<i>#co-induction principles#</i>#%}%.  Let us take that tack here, so that we can arrive at an [induction x; crush]-style proof for [ones_eq'].
+
+   An induction principle is parameterized over a predicate characterizing what we mean to prove, %\emph{%#<i>#as a function of the inductive fact that we already know#</i>#%}%.  Dually, a co-induction principle ought to be parameterized over a predicate characterizing what we mean to prove, %\emph{%#<i>#as a function of the arguments to the co-inductive predicate that we are trying to prove#</i>#%}%.
+
+   To state a useful principle for [stream_eq], it will be useful first to define the stream head function. *)
+
+Definition hd A (s : stream A) : A :=
+  match s with
+    | Cons x _ => x
+  end.
+
+(** Now we enter a section for the co-induction principle, based on %\index{Park's principle}%Park's principle as introduced in a tutorial by Gim%\'%enez%~\cite{IT}%. *)
+
+Section stream_eq_coind.
+  Variable A : Set.
+  Variable R : stream A -> stream A -> Prop.
+  (** This relation generalizes the theorem we want to prove, characterizinge exactly which two arguments to [stream_eq] we want to consider. *)
+
+  Hypothesis Cons_case_hd : forall s1 s2, R s1 s2 -> hd s1 = hd s2.
+  Hypothesis Cons_case_tl : forall s1 s2, R s1 s2 -> R (tl s1) (tl s2).
+  (** Two hypotheses characterize what makes a good choice of [R]: it enforces equality of stream heads, and it is %``%#<i>#hereditary#</i>#%''% in the sense that a [R] stream pair passes on %``%#"#[R]-ness#"#%''% to its tails.  An established technical term for such a relation is %\index{bisimulation}\emph{%#<i>#bisimulation#</i>#%}%. *)
+
+  (** Now it is straightforward to prove the principle, which says that any stream pair in [R] is equal.  The reader may wish to step through the proof script to see what is going on. *)
+  Theorem stream_eq_coind : forall s1 s2, R s1 s2 -> stream_eq s1 s2.
+    cofix; destruct s1; destruct s2; intro.
+    generalize (Cons_case_hd H); intro Heq; simpl in Heq; rewrite Heq.
+    constructor.
+    apply stream_eq_coind.
+    apply (Cons_case_tl H).
+  Qed.
+End stream_eq_coind.
+
+(** To see why this proof is guarded, we can print it and verify that the one co-recursive call is an immediate argument to a constructor. *)
+Print stream_eq_coind.
+
+(** We omit the output and proceed to proving [ones_eq''] again.  The only bit of ingenuity is in choosing [R], and in this case the most restrictive predicate works. *)
+
+Theorem ones_eq'' : stream_eq ones ones'.
+  apply (stream_eq_coind (fun s1 s2 => s1 = ones /\ s2 = ones')); crush.
+Qed.
+
+(** Note that this proof achieves the proper reduction behavior via [hd] and [tl], rather than [frob] as in the last proof.  All three functions pattern match on their arguments, catalyzing computation steps.
+
+   Compared to the inductive proofs that we are used to, it still seems unsatisfactory that we had to write out a choice of [R] in the last proof.  An alternate is to capture a common pattern of co-recursion in a more specialized co-induction principle.  For the current example, that pattern is: prove [stream_eq s1 s2] where [s1] and [s2] are defined as their own tails. *)
+
+Section stream_eq_loop.
+  Variable A : Set.
+  Variables s1 s2 : stream A.
+
+  Hypothesis Cons_case_hd : hd s1 = hd s2.
+  Hypothesis loop1 : tl s1 = s1.
+  Hypothesis loop2 : tl s2 = s2.
+
+  (** The proof of the principle includes a choice of [R], so that we no longer need to make such choices thereafter. *)
+
+  Theorem stream_eq_loop : stream_eq s1 s2.
+    apply (stream_eq_coind (fun s1' s2' => s1' = s1 /\ s2' = s2)); crush.
+  Qed.
+End stream_eq_loop.
+
+Theorem ones_eq''' : stream_eq ones ones'.
+  apply stream_eq_loop; crush.
+Qed.
 (* end thide *)
 
-(** The standard [auto] machinery sees that our goal matches an assumption and so applies that assumption, even though this violates guardedness.  One usually starts a proof like this by [destruct]ing some parameter and running a custom tactic to figure out the first proof rule to apply for each case.  Alternatively, there are tricks that can be played with %``%#"#hiding#"#%''% the co-inductive hypothesis. *)
+(** Let us put [stream_eq_ind] through its paces a bit more, considering two different ways to compute infinite streams of all factorial values.  First, we import the [fact] factorial function from the standard library. *)
+
+Require Import Arith.
+Print fact.
+(** %\vspace{-.15in}%[[
+fact = 
+fix fact (n : nat) : nat :=
+  match n with
+  | 0 => 1
+  | S n0 => S n0 * fact n0
+  end
+     : nat -> nat
+]]
+*)
+
+(** The simplest way to compute the factorial stream involves calling [fact] afresh at each position. *)
+
+CoFixpoint fact_slow' (n : nat) := Cons (fact n) (fact_slow' (S n)).
+Definition fact_slow := fact_slow' 1.
+
+(** A more clever, optimized method maintains an accumulator of the previous factorial, so that each new entry can be computed with a single multiplication. *)
+
+CoFixpoint fact_iter' (cur acc : nat) := Cons acc (fact_iter' (S cur) (acc * cur)).
+Definition fact_iter := fact_iter' 2 1.
+
+(** We can verify that the streams are equal up to particular finite bounds. *)
+
+Eval simpl in approx fact_iter 5.
+(** %\vspace{-.15in}%[[
+     = 1 :: 2 :: 6 :: 24 :: 120 :: nil
+     : list nat
+]]
+*)
+Eval simpl in approx fact_slow 5.
+(** %\vspace{-.15in}%[[
+     = 1 :: 2 :: 6 :: 24 :: 120 :: nil
+     : list nat
+]]
+
+Now, to prove that the two versions are equivalent, it is helpful to prove (and add as a proof hint) a quick lemma about the computational behavior of [fact]. *)
+
+(* begin thide *)
+Lemma fact_def : forall x n,
+  fact_iter' x (fact n * S n) = fact_iter' x (fact (S n)).
+  simpl; intros; f_equal; ring.
+Qed.
+
+Hint Resolve fact_def.
+
+(** With the hint added, it is easy to prove an auxiliary lemma relating [fact_iter'] and [fact_slow'].  The key bit of ingenuity is introduction of an existential quantifier for the shared parameter [n]. *)
+
+Lemma fact_eq' : forall n, stream_eq (fact_iter' (S n) (fact n)) (fact_slow' n).
+  intro; apply (stream_eq_coind (fun s1 s2 => exists n, s1 = fact_iter' (S n) (fact n)
+    /\ s2 = fact_slow' n)); crush; eauto.
+Qed.
+
+(** The final theorem is a direct corollary of [fact_eq']. *)
+
+Theorem fact_eq : stream_eq fact_iter fact_slow.
+  apply fact_eq'.
+Qed.
+
+(** As in the case of [ones_eq'], we may be unsatisfied that we needed to write down a choice of [R] that seems to duplicate information already present in a lemma statement.  We can facilitate a simpler proof by defining a co-induction principle specialized to goals that begin with single universal quantifiers, and the strategy can be extended in a straightforward way to principles for other counts of quantifiers.  (Our [stream_eq_loop] principle is effectively the instantiation of this technique to zero quantifiers.) *)
+
+Section stream_eq_onequant.
+  Variables A B : Set.
+  (** We have the types [A], the domain of the one quantifier; and [B], the type of data found in the streams. *)
+
+  Variables f g : A -> stream B.
+  (** The two streams we compare must be of the forms [f x] and [g x], for some shared [x].  Note that this falls out naturally when [x] is a shared universally quantified variable in a lemma statement. *)
+
+  Hypothesis Cons_case_hd : forall x, hd (f x) = hd (g x).
+  Hypothesis Cons_case_tl : forall x, exists y, tl (f x) = f y /\ tl (g x) = g y.
+  (** These conditions are inspired by the bisimulation requirements, with a more general version of the [R] choice we made for [fact_eq'] inlined into the hypotheses of [stream_eq_coind]. *)
+
+  Theorem stream_eq_onequant : forall x, stream_eq (f x) (g x).
+    intro; apply (stream_eq_coind (fun s1 s2 => exists x, s1 = f x /\ s2 = g x)); crush; eauto.
+  Qed.
+End stream_eq_onequant.
+
+Lemma fact_eq'' : forall n, stream_eq (fact_iter' (S n) (fact n)) (fact_slow' n).
+  apply stream_eq_onequant; crush; eauto.
+Qed.
+
+(** We have arrived at one of our customary automated proofs, thanks to the new principle. *)
+(* end thide *)
 
 
 (** * Simple Modeling of Non-Terminating Programs *)
@@ -378,7 +560,7 @@ Lemma exec_total : forall pc rs i,
     end; eauto.
 Qed.
 
-(** We are ready to define a co-inductive judgment capturing the idea that a program runs forever.  We define the judgment in terms of a program [prog], represented as a function mapping each label to the instruction found there.  That is, to simplify the proof, we consider only infinitely-long programs. *)
+(** We are ready to define a co-inductive judgment capturing the idea that a program runs forever.  We define the judgment in terms of a program [prog], represented as a function mapping each label to the instruction found there.  That is, to simplify the proof, we consider only infinitely long programs. *)
 
 Section safe.
   Variable prog : label -> instr.
@@ -389,7 +571,7 @@ Section safe.
     -> safe pc' r'
     -> safe pc r.
 
-  (** Now we can prove that any starting address and register bank lead to safe infinite execution.  Recall that proofs of existentially-quantified formulas are all built with a single constructor of the inductive type [ex].  This means that we can use [destruct] to %``%#"#open up#"#%''% such proofs.  In the proof below, we want to perform this opening up on an appropriate use of the [exec_total] lemma.  This lemma's conclusion begins with two existential quantifiers, so we want to tell [destruct] that it should not stop at the first quantifier.  We accomplish our goal by using an %\textit{%#<i>#intro pattern#</i>#%}% with [destruct].  Consult the Coq manual for the details of intro patterns; the specific pattern [[? [? ?]]] that we use here accomplishes our goal of destructing both quantifiers at once. *)
+  (** Now we can prove that any starting address and register bank lead to safe infinite execution.  Recall that proofs of existentially quantified formulas are all built with a single constructor of the inductive type [ex].  This means that we can use [destruct] to %``%#"#open up#"#%''% such proofs.  In the proof below, we want to perform this opening up on an appropriate use of the [exec_total] lemma.  This lemma's conclusion begins with two existential quantifiers, so we want to tell [destruct] that it should not stop at the first quantifier.  We accomplish our goal by using an %\textit{%#<i>#intro pattern#</i>#%}% with [destruct].  Consult the Coq manual for the details of intro patterns; the specific pattern [[? [? ?]]] that we use here accomplishes our goal of destructing both quantifiers at once. *)
   
   Theorem always_safe : forall pc rs,
     safe pc rs.
